src/rocq/Utils/CTreeUtils.v
@@ -1,0 +1,72 @@
+Unset Universe Checking.
+
+From CTree Require Import
+  CTree CTreeDefinitions Eq Fold FoldStateT.
+
+From ExtLib Require Import
+  Structures.Functor
+  Structures.Monads.
+
+Import Monad.
+
+#[global] Instance ctree_monad {E B} : Monad (ctree E B).
+split.
+- intros.
+  apply ret; apply X.
+- intros t u X X0.
+  eapply bind.
+  apply X.
+  apply X0.
+Defined.
+
+#[global] Instance ctree_eq1 {Eff B} : Monad.Eq1 (ctree Eff B).
+intros A.
+apply sbisim.
+apply eq.
+Defined.
+
+#[global] Instance ctree_monad_eq1_equiv {Eff B} : Monad.Eq1Equivalence (ctree Eff B).
+red.
+typeclasses eauto.
+Defined.
+
+#[global] Instance ctree_monad_laws {E B} : MonadLawsE (ctree E B).
+split.
+- (* bind_ret_l *)
+  intros A B0 f x.
+  setoid_rewrite Equ.bind_ret_l.
+  reflexivity.
+- (* bind_ret_r *)
+  intros A x.
+  setoid_rewrite Equ.bind_ret_r.
+  reflexivity.
+- (* bind_bind *)
+  intros A B0 C x f g.
+  setoid_rewrite Equ.bind_bind.
+  reflexivity.  
+- typeclasses eauto.
+Defined.
+
+#[global] Instance MonadStepState {S M} `{HM : Monad M} `{MS : MonadStep M} : MonadStep (Monads.stateT S M).
+red.
+intros s.
+eapply bind.
+apply mstep.
+intros _.
+apply (ret (s, tt)).
+Defined.
+
+#[global] Instance MonadStuckState {S M} `{HM : Monad M} `{MS : MonadStuck M} : MonadStuck (Monads.stateT S M).
+red.
+intros X.
+red.
+intros s.
+apply mstuck.
+Defined.
+
+#[global] Instance MonadBrState {B S M} `{HM : Monad M} `{MB : MonadBr B M} : MonadBr B (Monads.stateT S M).
+red.
+intros X b s.
+apply mbr in b.
+eapply fmap; cycle 1; eauto.
+Defined.
